Re-factor codes, rename, and remove unnecessary  files

Strand_library.v
@@ -1,19 +1,638 @@
 
-(* This file contains all basic results for Coq which will be used when proving *)
+(* This file contains all basic results for strand spaces which will be used when proving *)
 
 Require Import Lists.List Omega.
+Require Import Strand_Spaces Message_Algebra.
+Require Import ProofIrrelevance.
+Require Import Relation_Definitions Relation_Operators.
+Require Import Classical.
 
-Lemma nth_error_len : 
-  forall (A:Type) (l:list A) (n:nat), nth_error l n = None -> (length l) <= n.
+Import ListNotations.
+
+Lemma nth_error_some_In {X:Type}: forall l i (x:X),
+nth_error l i = Some x ->
+List.In x l.
 Proof.
-intros A l n. generalize dependent l.
-induction n.
-intros l H.
-unfold nth_error in H.
-unfold error in H. destruct l. auto. inversion H.
+  intros l. induction l.
+  intros i x nth. destruct i. simpl in nth; inversion nth.
+  simpl in nth; inversion nth.
+  intros i x nth.
+  destruct i. simpl in nth. inversion nth. left. reflexivity.
+  simpl in nth. right. eapply IHl. exact nth.
+Qed.
+Hint Resolve nth_error_some_In.
 
-intros l1 H. destruct l1. simpl; omega.
-inversion H. apply IHn in H. simpl. omega.
+ Lemma nth_error_node : forall n,
+nth_error (strand_of n) (index_of n) = Some (smsg_of n).
+Proof.
+  intros n.
+  unfold smsg_of. destruct valid_smsg. 
+  destruct n. simpl in *.
+  destruct x0. simpl. auto.
+Qed.
+Hint Resolve nth_error_node.
+
+Lemma strand_node : forall (s: strand) (i: nat),
+i < length s ->
+exists n, strand_of n = s /\ index_of n = i.
+Proof.
+  intros s i len.  
+  eexists (exist _ (s,i) _). simpl.
+  split; reflexivity.
+  Grab Existential Variables.
+  simpl. exact len.
+Qed.
+Hint Resolve strand_node.
+
+(** Every signed message of a node must be some signed message
+in the node's strand %\\%*)
+Lemma smsg_in_strand : forall n s,
+(strand_of n) = s ->
+List.In (smsg_of n) s.
+Proof.
+  intros.
+  eapply nth_error_some_In. subst.
+  apply nth_error_node. 
+Qed. 
+
+(** ** xmit and recv *)
+
+(** No node is both transmit and receive %\\% *)
+Lemma xmit_vs_recv: forall (n:node),  xmit(n) -> recv(n) -> False.
+Proof.
+intros n Hx Hr.
+inversion Hx. inversion Hr.
+rewrite H in H0. discriminate.
 Qed.
 
+(** every  node is either transmit or receive %\\% *)
+Lemma xmit_or_recv: forall (n: node), xmit n \/ recv n.
+Proof.
+intros n. unfold xmit, recv. case (smsg_of n).
+intros. left. exists m. auto.
+intros. right. exists m. auto.
+Qed.
+
+(** strand-successor is irreflexive %\\% *)
+Lemma ssucc_not_ref: forall (n:node),  ssucc n n -> False.
+Proof.
+intros n Hs. inversion Hs. destruct H. omega.
+Qed.
+
+(* TODO : move to right place *)
+Lemma eq_nodes : forall (x y : node), strand_of(x) = strand_of(y) -> 
+  index_of(x) = index_of(y) -> x = y.
+Proof.
+  intros [[xs xn] xp] [[ys yn] yp] eq_index eq_strand.
+  simpl in eq_index, eq_strand. subst.
+  rewrite (proof_irrelevance (lt yn (length ys)) xp yp). reflexivity.
+Qed.
+
+
+Lemma node_smsg_msg_xmit : forall n t,
+smsg_of(n) = (+ t) ->
+msg_of(n) = t.
+Proof.
+  intros n t H.
+  unfold msg_of. rewrite H. reflexivity. 
+Qed.
+Hint Resolve node_smsg_msg_xmit.
+
+Lemma node_smsg_msg_recv : forall n t,
+smsg_of(n) = (- t) ->
+msg_of(n) = t.
+Proof.
+  intros n t H.
+  unfold msg_of. rewrite H. reflexivity. 
+Qed.
+Hint Resolve node_smsg_msg_recv.
+
+(** strand-successors are unique %\\% *)
+Lemma ssucc_unique: 
+  forall (x y z: node),  ssucc x y -> ssucc x z  -> y = z.
+Proof.
+  intros x y z Hxy Hxz.
+  destruct Hxy, Hxz.
+  apply eq_nodes; destruct H, H0; try omega; congruence.
+Qed.
+Hint Resolve ssucc_unique.
+
+(** Every node and its successor are on the same strand %\\%*)
+Lemma ssucc_same_strand :
+  forall (x y : node), ssucc x y -> strand_of(x) = strand_of(y).
+Proof.
+intros x y Sxy. inversion Sxy. destruct H; auto.
+Qed.
+Hint Resolve ssucc_same_strand. 
+
+(** Lemma for strand_of *)
+Lemma ssuccs_same_strand :
+  forall (x y : node), ssuccs x y -> strand_of x = strand_of y.
+Proof.
+  intros x y Sxy.
+  induction Sxy.
+  auto. congruence.
+Qed.
+Hint Resolve ssuccs_same_strand.
+
+(** ** Baby result about msg_deliver *)
+Lemma msg_deliver_xmit : forall x y, msg_deliver x y -> xmit x.
+Proof.
+intros x y Md.
+destruct Md. 
+unfold xmit. exists m; apply H.
+Qed.
+
+Lemma msg_deliver_recv : forall x y, msg_deliver x y -> recv y.
+Proof.
+intros x y Md.
+destruct Md.
+unfold recv. exists m; apply H.
+Qed.
+
+(** ** Baby results about prec *)
+
+Theorem prec_transitive:
+  forall x y z, (prec x y) -> (prec y z) -> (prec x z).
+Proof.
+  apply t_trans.
+Qed.
+
+Lemma deliver_prec:
+  forall x y, (msg_deliver x y) -> (prec x y).
+Proof.
+  intros. constructor. constructor. auto.
+Qed.
+
+Lemma ssucc_prec:
+  forall x y, (ssucc x y) -> (prec x y).
+Proof.
+  intros. constructor. apply edge_double. auto.
+Qed.
+
+
+Lemma ssuccs_prec:
+  forall x y, (ssuccs x y) -> (prec x y).
+Proof.
+  intros x y Sxy.
+  induction Sxy.
+  apply ssucc_prec; auto.
+  apply prec_transitive with (y:=y); auto.
+Qed.
+
+(** ** Basic Results for Penetrator Strands *)
+  Lemma strand_1_node : forall n x, strand_of n = [x] -> smsg_of n = x.
+  Proof.
+  intros n x Snx.
+  assert (H : List.In (smsg_of n) [x]).
+  apply smsg_in_strand; auto.
+  elim H; auto.
+  intro. elim H0.
+  Qed.
+
+(* If n is a node of a MStrand or KStrand, then n is a positive node *)
+  Lemma MStrand_xmit_node : 
+    forall (n:node), MStrand (strand_of n) -> xmit n.
+  Proof.
+    unfold xmit.
+    intros n Ms. inversion Ms. exists (T t).
+    apply strand_1_node. auto.
+  Qed.
+
+  Lemma KStrand_xmit_node :
+    forall (n:node), KStrand (strand_of n) -> xmit n.
+  Proof.
+    unfold xmit.
+    intros n Ms. inversion Ms. exists (K k).
+    apply strand_1_node. auto.
+  Qed.
+
+  Lemma strand_3_nodes :
+    forall n x y z, strand_of n = [x;y;z] ->
+    smsg_of n = x \/ smsg_of n = y \/ smsg_of n = z.
+  Proof.
+    intros n x y z Sxyz.
+    assert (Lxyz : List.In (smsg_of n) [x;y;z]) .
+    apply smsg_in_strand; auto.
+    elim Lxyz. auto.
+    intro Lyz. elim Lyz; auto.
+    intro Lz. elim Lz; auto.
+    intro Le. elim Le; auto.
+  Qed.
+
+  Lemma strand_3_nodes_nnp_xmit :
+   forall n x y z, strand_of n = [-x;-y;+z] -> xmit n -> smsg_of n = +z.
+  Proof.
+  intros n x y z Sxyz Xn.
+  assert (Hxyz : smsg_of n = -x \/ smsg_of n = -y \/ smsg_of n = +z).
+  apply strand_3_nodes. auto.
+  case Hxyz. intro. apply False_ind. apply (xmit_vs_recv n).
+    auto. unfold recv; auto; exists x; auto.
+  intros Hyz. case Hyz. intro. apply False_ind. apply (xmit_vs_recv n).
+    auto. unfold recv; auto; exists y; auto.
+  auto.
+  Qed.
+
+  Lemma strand_3_nodes_nnp_recv :
+   forall n x y z, strand_of n = [-x;-y;+z] -> recv n -> 
+   smsg_of n = -x \/ smsg_of n = -y.
+  Proof.
+  intros n x y z Sxyz Xn.
+  assert (Hxyz : smsg_of n = -x \/ smsg_of n = -y \/ smsg_of n = +z).
+  apply strand_3_nodes. auto.
+  case Hxyz. intro. left; auto.
+  intro Hyz. case Hyz. right; auto.
+  intro Hz. apply False_ind. apply (xmit_vs_recv n).
+    unfold xmit. exists z ; auto. auto.
+  Qed.
+
+  Lemma strand_3_nodes_npp_recv :
+   forall n x y z, strand_of n = [-x;+y;+z] -> recv n -> 
+   smsg_of n = -x.
+  Proof.
+  intros n x y z Sxyz Xn.
+  assert (Hxyz : smsg_of n = -x \/ smsg_of n = +y \/ smsg_of n = +z).
+  apply strand_3_nodes. auto.
+  case Hxyz. intro. auto.
+  intro Hyz. case Hyz. intro. apply False_ind. apply (xmit_vs_recv n).
+    unfold xmit. exists y. auto. auto.
+  intro Hz. apply False_ind. apply (xmit_vs_recv n).
+    unfold xmit. exists z ; auto. auto.
+  Qed.
+
+  (** TODO : move to right place *)
+  Lemma pair_not_ingred_comp_l : forall x y, ~(P x y) <st x.
+  Proof.
+    intros x y Hingred.
+    assert (Hlt : size (P x y ) <= size x).
+    apply ingred_lt. auto.
+    assert (Hgt : size (P x y) > size x).
+    simpl. apply size_lt_plus_l. omega.
+  Qed.
+
+  Lemma pair_not_ingred_comp_r :
+    forall x y, ~(P x y) <st y.
+  Proof.
+    intros x y Hst.
+    assert (Hlt : size (P x y ) <= size y).
+    apply ingred_lt. auto.
+    assert (Hgt : size (P x y) > size y).
+    simpl. rewrite (plus_comm (size x) (size y)).
+    apply size_lt_plus_l. omega.
+  Qed.
+
+  Lemma enc_not_ingred_comp_l : forall x y, ~(E x y) <st x.
+  Proof.
+    intros x y Hingred.
+    assert (Hlt : size (E x y ) <= size x).
+    apply ingred_lt. auto.
+    assert (Hgt : size (E x y) > size x).
+    simpl. omega. omega.
+  Qed.
+
+  Lemma enc_not_ingred_comp_r :
+    forall x y, ~(E x y) <st (K y).
+  Proof.
+    intros x y Hst.
+    assert (Hlt : size (E x y ) <= size (K y)).
+    apply ingred_lt. auto.
+    assert (Hgt : size (E x y) > size (K y)).
+    simpl. admit. (* TODO : Prove *)
+    omega.
+  Qed.
+  
+  Lemma CStrand_not_falling : 
+    forall (s:strand), CStrand s -> 
+      ~ exists (n1 n2 : node), recv n1 /\ xmit n2 /\ 
+        strand_of n1 = s /\ strand_of n2 = s /\ 
+        ingred (msg_of n2) (msg_of n1).
+  Proof.
+  intros s Hcs Hc.
+  destruct Hc as (n1,(n2,(Hre, (Hxmit,(Hs1,(Hs2,Hingred)))))).
+  inversion Hcs.
+  assert (Smn2 : smsg_of n2 = + P g h).
+   apply strand_3_nodes_nnp_xmit with (x:=g) (y:=h).
+   congruence. auto.
+  assert (Mn2 : msg_of n2 = P g h). unfold msg_of. rewrite Smn2. auto.
+  assert (Smn1 : smsg_of n1 = -g \/ smsg_of n1 = -h).
+    apply strand_3_nodes_nnp_recv with (x:=g) (y:=h) (z:=P g h).
+    congruence. auto.
+  case Smn1.
+    intro Sg. assert (Mn1 : msg_of n1 = g). unfold msg_of. rewrite Sg; auto.
+    apply (pair_not_ingred_comp_l g h). rewrite Mn1, Mn2 in Hingred. auto.
+    intro Sh. assert (Mn1 : msg_of n1 = h). unfold msg_of. rewrite Sh; auto.
+    apply (pair_not_ingred_comp_r g h). rewrite Mn1, Mn2 in Hingred. auto. 
+  Qed.
+
+  Lemma EStrand_not_falling : 
+    forall (s:strand), EStrand s -> 
+      ~ exists (n1 n2 : node), recv n1 /\ xmit n2  /\ 
+        strand_of n1 = s /\ strand_of n2 = s /\ 
+        ingred (msg_of n2) (msg_of n1).
+  Proof.
+  intros s Hes Hc.
+  destruct Hc as (n1,(n2,(Hre, (Hxmit,(Hs1,(Hs2,Hingred)))))).
+  inversion Hes.
+  assert (Smn2 : smsg_of n2 = + E h k).
+   apply strand_3_nodes_nnp_xmit with (x:=K k) (y:=h).
+   congruence. auto.
+  assert (Mn2 : msg_of n2 = E h k). unfold msg_of. rewrite Smn2. auto.
+  assert (Smn1 : smsg_of n1 = -K k \/ smsg_of n1 = -h).
+    apply strand_3_nodes_nnp_recv with (x:=K k) (y:=h) (z:=E h k).
+    congruence. auto.
+  case Smn1.
+    intro Sg. assert (Mn1 : msg_of n1 = K k). unfold msg_of. rewrite Sg; auto.
+    apply (enc_not_ingred_comp_r h k). rewrite Mn1, Mn2 in Hingred. auto.
+    intro Sh. assert (Mn1 : msg_of n1 = h). unfold msg_of. rewrite Sh; auto.
+    apply (enc_not_ingred_comp_l h k). rewrite Mn1, Mn2 in Hingred. auto.
+  Qed.
+
+(* (** ** Baby results about xmit and recv *)
+
+Lemma xmit_not_recv: forall n, xmit n -> ~(recv n).
+Proof.
+  intros.
+  unfold not.
+  intros.
+  apply xmit_vs_recv with (n:=n).
+  tauto.
+Qed.
+
+Lemma recv_not_xmit: forall n, recv n -> ~(xmit n).
+Proof.
+  intros n0 H0 H.
+  apply xmit_vs_recv with (n:=n0).
+  tauto.
+Qed.
+
+Lemma not_xmit_recv: forall n,  ~(xmit n) -> (recv n).
+Proof.
+  unfold not.
+  intro.
+  assert (a1: (xmit n \/ recv n)).
+  exact (xmit_or_recv n).
+  tauto.
+Qed.
+
+Lemma not_recv_xmit: forall n,  ~(recv n) -> (xmit n).
+Proof.
+  unfold not.
+  intro.
+  assert (a1: (xmit n \/ recv n)).
+  exact (xmit_or_recv n).
+  tauto.
+Qed.
+*)
+
+(*
+(** ** Baby results about origination
+   Some of these would be axioms, in a first-order axiomatization 
+*)
+
+(* (these are ugly proofs, I'm just flailing around) :*) 
+
+Lemma
+  orig_is_sent :
+  forall (n : node) (m : msg), orig_at n m ->  (ingred m (msg_of n)).
+
+Proof.
+  unfold orig_at.
+  tauto.
+Qed.
+
+Lemma
+  non_not_originate :
+  forall (n : node) (m : msg), non_orig m -> orig_at n m -> False.
+Proof.
+  intros n0 m0 H0.
+  unfold non_orig in H0.
+  intros H1.
+  unfold orig_at in H1.
+  destruct H1.
+  destruct H1.
+  assert (a0: orig_at n0 m0).
+  unfold orig_at.
+  auto.
+  assert (na0: ~ (orig_at n0 m0)).
+  apply H0.
+  tauto.
+Qed.
+
+
+Lemma
+  unique_only_once :
+  forall (m : msg) (n n' : node),
+    unique m -> orig_at n m -> orig_at n' m -> n = n'.
+Proof.
+  intros.
+  unfold unique in  H.
+  destruct H.
+  apply H2.
+  tauto.
+Qed.
+
+Lemma
+  orig_not_sent_earlier :
+  forall (n n' : node) (m : msg),
+    (orig_at n m) ->  (ssucc n' n) ->  (ingred m (msg_of n')) -> False.
+Proof.
+  intros n0 n'0 m0 H0.
+  intros H1.
+  intros H2.
+  unfold orig_at in H0.
+  destruct H0.
+  destruct H0.
+  apply (H3 n'0).
+  apply (ssuccs_step); auto.
+  auto.
+Qed.
+
+Lemma
+  unique_does_originate :
+  forall m : msg, unique m -> exists n : node, orig_at n m.
+Proof.
+  intros.
+  unfold unique in H.
+  destruct H.
+  destruct H.
+  exists x. auto.
+Qed.
+
+Lemma msg_deliver_prec:
+  forall n0 n1, (msg_deliver n0 n1) -> (prec n0 n1).
+Proof.
+  intros.
+  apply prec_msg_step; auto.
+Qed.
+*)
+(** ** Every inhabited predicate has a prec-minimal element *)
+Theorem always_min_elt :  forall P: node-> Prop, 
+  (exists (x:node), (P x)) -> has_min_elt P.
+Proof.
+  intros.
+  destruct H.
+  revert x H.
+  unfold has_min_elt.
+  unfold is_minimal.
+  apply (@well_founded_ind node prec (wf_prec)
+    (fun x:node =>
+      P x -> exists y:node, P y /\ (forall z:node, prec z y  ->   ~ (P z) ))).
+  intros.
+  case (classic (forall y:node, P y -> ~ prec y x)).
+  intros.
+  exists x.
+  split.
+  auto.
+  intros.
+  assert (a2: P z -> ~ prec z x).
+  apply H1.
+  tauto.
+  intros.
+  apply not_all_ex_not in H1.
+  destruct H1.
+  apply imply_to_and in H1.
+  destruct H1.
+  apply NNPP in H2.
+  apply H with (y:=x0).
+  assumption.
+  assumption.
+Qed.
+
+(** ** prec is acyclic *)
+
+Theorem prec_is_acyclic: forall (x:node), (prec x x) -> False.
+Proof.
+  intros x H.
+  assert (has_min_elt (fun x => prec x x )).
+  apply always_min_elt.
+  exists x;  auto.
+  unfold has_min_elt in H0.
+  destruct H0.
+  destruct H0.
+  assert (prec x0 x0 -> ~ prec x0 x0 ).
+  apply H1.
+  tauto.
+Qed.
+
+(** * Ingredients must originate *)
+
+Section IngredientsOriginate.
+
+  Variable the_m: msg.
+  Definition m_ingred (n: node): Prop := ingred the_m (msg_of n).
+
+(** If m is an ingredient somewhere then there is a minimal such place *)
+
+  Lemma 
+    ingred_min:
+    (exists n:node,  (m_ingred n)) ->
+    (exists n:node, (is_minimal m_ingred n)).
+  Proof.  
+    intros H.
+    apply always_min_elt; auto.
+  Qed.
+
+(** TODO : *)
+Lemma smsg_xmit_msg : 
+  forall n m, smsg_of(n) = (+ m) -> msg_of(n) = m.
+Proof.
+  intros n m H.
+  unfold msg_of. rewrite H. reflexivity. 
+Qed.
+Hint Resolve smsg_xmit_msg.
+
+Lemma smsg_recv_msg : 
+  forall n m, smsg_of(n) = (- m) -> msg_of(n) = m.
+Proof.
+  intros n m H.
+  unfold msg_of. rewrite H. reflexivity. 
+Qed.
+
+Hint Resolve smsg_recv_msg.
+
+Lemma msg_deliver_msg_eq : 
+  forall x y, x --> y -> msg_of x = msg_of y.
+Proof.
+  intros x y edge.
+  destruct edge. destruct H as (H1, (H2, H3)).
+  assert (msg_of(x) = m). apply smsg_xmit_msg. auto.
+  assert (msg_of(y) = m). apply smsg_recv_msg. auto.
+  congruence.
+Qed.
  
+(** A minimal node can't be a reception *)
+
+  Lemma
+    minimal_not_recv:
+    forall (n:node), (is_minimal m_ingred n) ->
+      ~ (recv n).
+  Proof.
+    unfold not.
+    intros.
+    unfold is_minimal in H.
+    destruct H.
+    assert (a1: exists n1, msg_deliver n1 n).
+    apply was_sent; auto.
+
+    destruct a1.
+    assert (a2: prec x n).
+    apply deliver_prec; auto.
+
+    assert (a3: ~(m_ingred x)).
+    apply H1; auto.
+    assert (a4: m_ingred x).
+
+    assert (a5: msg_of x = msg_of n).
+    apply msg_deliver_msg_eq. auto.
+    unfold m_ingred.
+    unfold m_ingred in H.
+    rewrite a5; auto.
+    tauto.
+  Qed.
+
+(** So, a minimal node must be a transmission *)
+
+  Lemma minimal_is_xmit:   forall (n:node), (is_minimal m_ingred n) ->
+    (xmit n).
+  Proof.
+    intros.
+    case (xmit_or_recv n). auto.
+    intro. apply False_ind. apply (minimal_not_recv n); auto.
+  Qed.
+
+
+
+(** Main result of this section: an ingredient must originate *)
+
+  Theorem
+    ingred_originates_2:
+    (exists n:node, (ingred the_m (msg_of n))) ->
+    (exists n:node, (orig_at n the_m)).
+  Proof.
+    intros.
+    assert (a1: has_min_elt m_ingred).
+    apply always_min_elt.
+    unfold m_ingred; auto.
+    unfold orig_at.
+    unfold has_min_elt in a1.
+    destruct a1.
+    assert (a0: xmit x).
+    apply minimal_is_xmit; auto.
+
+    unfold m_ingred in H0.
+    unfold is_minimal in H0.
+    destruct H0.
+    exists x.
+    split.
+    auto.
+    split.
+    auto.
+    intros.
+    assert (a1: prec n' x).
+    apply ssuccs_prec; auto.
+    revert H3.
+    unfold not in H1.
+    apply H1; auto.
+  Qed.
+
+End IngredientsOriginate.
