Authentication_Tests_Library.v
@@ -1,0 +1,192 @@
+
+(* This file contains all the propositions needed for authentication tets *)
+
+Require Import Strand_Spaces Message_Algebra Strand_Library.
+Require Import Lists.List.
+
+(** * Proposition 7 *)
+Section P7_1.
+  Variable i : nat.
+  Variable p : list node.
+  Let p_i := nth_node i p.
+  Let p_i1 := nth_node (i+1) p.
+  Hypothesis Hc : 0 < i /\ i < length p - 1.
+  Hypothesis Hfp : falling_path p.
+  Hypothesis Hrec : recv p_i.
+  Hypothesis Hpn : p_node p_i.
+  Let s := strand_of p_i.
+
+  Lemma path_edge_pi_pi1 : path_edge p_i p_i1.
+  Proof.
+  destruct Hfp as (Hp,_). destruct Hp as (P, _).
+  unfold is_path in P.
+  apply (P i); apply Hc.
+  Qed.
+
+  Lemma P7_1_aux1 : xmit p_i1 /\ strand_of p_i1 = strand_of p_i.
+  Proof.
+  assert (Pe : path_edge p_i p_i1).
+  apply path_edge_pi_pi1; auto.
+  inversion Pe. apply False_ind. apply xmit_vs_recv with (n:=p_i).
+  apply msg_deliver_xmit with (y:=p_i1). auto. auto.
+  split. apply H.
+  destruct H. symmetry. apply ssuccs_same_strand. auto.
+  Qed.
+  
+  Lemma pi1_ingred_pi : msg_of p_i1 <st msg_of p_i.
+  Proof.
+  destruct Hfp. apply (H0 i). apply Hc.
+  Qed.
+
+  Lemma P7_1_aux : DStrand (strand_of p_i) \/ SStrand (strand_of p_i).
+  Proof.
+    assert (Ps : PenetratorStrand s). apply Hpn. 
+    inversion Ps. 
+    apply False_ind. apply xmit_vs_recv with (n:=p_i).
+      apply MStrand_xmit_node; auto. auto.
+    
+    apply False_ind. apply xmit_vs_recv with (n:=p_i).
+      apply KStrand_xmit_node; auto. auto.
+   
+    apply False_ind. apply (CStrand_not_falling s) ; auto.
+      exists p_i, p_i1. split; auto. split. apply P7_1_aux1.
+      split; auto. split. apply P7_1_aux1. apply pi1_ingred_pi.
+
+    auto.
+
+    apply False_ind. apply False_ind. apply (EStrand_not_falling s) ; auto.
+      exists p_i, p_i1. split; auto. split. apply P7_1_aux1.
+      split; auto. split. apply P7_1_aux1. apply pi1_ingred_pi.
+
+    auto.
+    Qed.  
+
+Section P7_1_a.
+  Variable h : msg.
+  Variable k : Key.
+  Hypothesis Heq : msg_of p_i = E h k.
+  Lemma P7_1a : 
+    DStrand s /\ msg_of p_i1 = h.
+  Proof.
+    case P7_1_aux.
+    intro Ds. split; auto.
+    inversion Ds.
+    assert (Smpi : smsg_of p_i = - K k' \/ smsg_of p_i = - E h0 k0).
+      apply strand_3_nodes_nnp_recv with (z:=h0); auto.
+      case Smpi. intro Kk. assert (msg_of p_i = K k').
+      unfold msg_of. rewrite Kk; auto. rewrite H1 in Heq. discriminate.
+   intro. assert (msg_of p_i = E h0 k0). unfold msg_of; rewrite H1; auto.
+     rewrite Heq in H2. assert (h=h0 /\ k = k0). apply ((enc_free h k h0 k0)); auto.
+     destruct H3; subst.
+     apply node_smsg_msg_xmit. 
+     apply strand_3_nodes_nnp_xmit with (x:= K k') (y:=E h0 k0). 
+     assert (strand_of p_i1 = strand_of p_i). apply P7_1_aux1. congruence.
+     apply P7_1_aux1.
+  intro. inversion H.
+    assert (smsg_of p_i = - P g h0). 
+    apply strand_3_nodes_npp_recv with (y:= g) (z:=h0). auto. auto.
+    assert (msg_of p_i= P g h0). apply node_smsg_msg_recv; auto. 
+    rewrite H2 in Heq. discriminate.
+  Qed.
+
+End P7_1_a.
+
+Section P7_1_b.
+  Variable g h : msg.
+  Lemma P7_1_b : 
+    SStrand s /\ (msg_of p_i1 = h \/ msg_of p_i1 = g).
+Admitted.
+End P7_1_b.
+End P7_1.
+
+(*********************************************************************)
+
+(** * Proposition 10 *)
+Section Proposition_10.
+  Variable p : path.
+  Variable n : nat.
+  Hypothesis Htp : is_trans_path p.
+  Hypothesis Hn : n < length p - 1.
+  Hypothesis Hcom : L p n <> L p (n+1).
+
+  Lemma ssuccs_eq : 
+    forall x y z, ssuccs x y -> ssuccseq y z -> ssuccs x z.
+  Admitted.
+
+  Lemma trans_path_ssuccs : 
+      ssuccs (nd p n) (nd p (n+1)) /\ recv (nd p n) /\ xmit (nd p (n+1)). 
+  Proof.
+    unfold is_trans_path in Htp.
+    destruct Htp as ((H3,H4),H5).
+    remember (H5 n) as H6.
+    destruct H6 as (H61, H62).
+    remember (H62 Hn) as H7.
+    case H7.
+    intros. apply False_ind. apply Hcom. auto.
+    intros. remember (H Hcom) as H8.
+    destruct H8 as (Hrec, (Hxmit, (Hss, (m, (H9, (H10, (H11, H12))))))).
+    repeat split.
+    apply ssuccs_eq with (y:= m); auto.
+    auto.
+    auto.
+  Qed.
+(*
+  Lemma Proposition_10 : p_node (nd p n) -> ssuccs (nd p n) (nd p (n+1)) /\ 
+    (DStrand (strand_of (nd p n)) \/ EStrand (strand_of (nd p n))).
+  Proof.
+    intro Hpn. 
+    assert (Hs : ssuccs (nd p n) (nd p (n + 1)) /\ recv (nd p n) /\ xmit (nd p (n+1))).
+    apply trans_path_ssuccs; auto.
+    unfold is_trans_path in Htp.
+    destruct Htp as (Ha, Hb).
+    split.
+    apply Hs.
+    
+    assert (Hp : PenetratorStrand (strand_of (nd p n))).
+    apply (P_node_strand (nd p n)); auto.
+    elim Hp.
+    intro. apply False_ind. apply (MStrand_not_edge (strand_of (nd p n))).
+    auto.
+    exists (nd p n).
+    exists (nd p (n+1)).
+    split. auto.
+    split. symmetry. apply ssuccs_same_strand. apply Hs.
+    apply Hs.
+
+    intro. apply False_ind. apply (KStrand_not_edge (strand_of (nd p n))).
+    auto.
+    exists (nd p n).
+    exists (nd p (n+1)).
+    split. auto.
+    split. symmetry. apply ssuccs_same_strand; apply Hs.
+    apply Hs.
+
+    intro. apply False_ind. apply (CStrand_not (strand_of (nd p n))).
+    auto.
+    exists (nd p n).
+    exists (nd p (n+1)).
+    split. auto.
+    split. symmetry. apply ssuccs_same_strand. apply Hs.
+    repeat split. apply Hs. apply Hs. apply Hs.
+    exists (L p n). exists (L p (n+1)).
+    split. apply Hb. omega.
+    split. apply Hb with (n:= n+1). omega.
+    auto.
+
+    intro. apply False_ind. apply (SStrand_not (strand_of (nd p n))).
+    auto.
+    exists (nd p n).
+    exists (nd p (n+1)).
+    split. auto.
+    split. symmetry. apply ssuccs_same_strand. apply Hs.
+    repeat split. apply Hs. apply Hs. apply Hs.
+    exists (L p n). exists (L p (n+1)).
+    split. apply Hb. omega.
+    split. apply Hb with (n:= n+1). omega.
+    auto.
+
+    auto.
+    auto.
+  Qed.
+*)
+End Proposition_10.
